cleanup in checkDecodeBoolList

theories/TM/Code/DecodeList.v
@@ -1,4 +1,5 @@
 From Undecidability.TM Require Import TM ProgrammingTools Code.
+From Undecidability.TM Require Hoare.
 From Complexity.TM Require Import Code.Decode.
 Require Import FunInd Lia Ring Arith Program.Wf.
 
@@ -28,8 +29,8 @@ Qed. *)
 
 From Complexity.TM Require Import Code.DecodeBool.
 
-Module CheckEncodeList.
-  Section checkEncodeList.
+Module CheckEncodesBoolList.
+  Section checkEncodesBoolList.
 
     (* Context (sigX:finType) X (cX : codable sigX X). *)
     Local Notation sigX := bool (only parsing).
@@ -44,10 +45,10 @@ Module CheckEncodeList.
     
     Local Remove Hints Retract_id : typeclass_instances.
     
-    Let Rel : pRel tau bool 1 := ContainsEncoding.Rel (Encode_list cX) Retr_f.
+    Let Rel' : pRel tau bool 1 := ContainsEncoding.Rel (Encode_list cX) Retr_f.
     Let Rel__X :=  ContainsEncoding.Rel (tau:=tau) cX Retr_f.
     
-    Definition R__step : pRel tau (option bool) 1 :=
+    Definition R'__step : pRel tau (option bool) 1 :=
       fun t '(y,t') =>
         match Option.bind Retr_g (current t[@Fin0]) with
           Some sigList_nil => t[@Fin0]=t'[@Fin0]
@@ -67,7 +68,7 @@ Module CheckEncodeList.
     Local Notation M__X := (CheckEncodesBool.M (I:=I__X)) (only parsing).
     Local Notation Realises__X := (RealiseIn_Realise (@CheckEncodesBool.RealisesIn _ _)) (only parsing).
     
-    Definition M__step : pTM tau (option bool) 1 :=
+    Definition M'__step : pTM tau (option bool) 1 :=
       Switch (Relabel ReadChar (Option.bind Retr_g))
              (fun c =>
                 match c with
@@ -76,9 +77,9 @@ Module CheckEncodeList.
                 | _ => Return Nop (Some false)
                 end).
     
-    Lemma Realises__step: M__step ⊨ R__step.
+    Lemma Realises'__step: M'__step ⊨ R'__step.
     Proof.
-      unfold M__step,R__step.
+      unfold M'__step,R'__step.
       eapply Realise_monotone.
       { eapply Switch_Realise. now TM_Correct.
         introsSwitch c. destructBoth c as [ [] | ]. all:TM_Correct. apply Realises__X. }
@@ -90,10 +91,10 @@ Module CheckEncodeList.
       destruct H as (t2&(?&->)&?&_&Ht2&->&_&<-). eexists t2,true. hnf in t2. destruct_vector. cbn.  easy.
     Qed.
                
-    Lemma Terminates__step T__X (Ter__X : projT1 M__X ↓ T__X):
-      projT1 M__step ↓  (fun t k => exists k', T__X ([|tape_move_right t[@Fin0]|]) k' /\ k' + 7 <= k ).
+    Lemma Terminates'__step T__X (Ter__X : projT1 M__X ↓ T__X):
+      projT1 M'__step ↓  (fun t k => exists k', T__X ([|tape_move_right t[@Fin0]|]) k' /\ k' + 7 <= k ).
     Proof.
-      unfold M__step.
+      unfold M'__step.
       eapply TerminatesIn_monotone.
       { eapply Switch_TerminatesIn. 1,2:now TM_Correct.
         introsSwitch c. destructBoth c as [ [] | ]. all:TM_Correct. all:try eassumption. eapply RealiseIn_Realise, CheckEncodesBool.RealisesIn. }
@@ -107,17 +108,17 @@ Module CheckEncodeList.
       } ring_simplify. nia.
     Qed.
 
-    Definition M := While M__step.
+    Definition M' := While M'__step.
 
-    Lemma Realise:
+    Lemma Realise':
       (*prefixInjective cX -> *)
       (forall (x:X), encode x <> []) ->
-      M ⊨ Rel.
+      M' ⊨ Rel'.
     Proof.
-      intros (*EpI_cX *) Hnnil. unfold Rel. 
+      intros (*EpI_cX *) Hnnil. unfold Rel'. 
       eapply Realise_monotone.
-      { unfold M. TM_Correct_step. eapply Realises__step. }
-      apply WhileInduction. all:unfold R__step,Rel;cbn.
+      { unfold M'. TM_Correct_step. eapply Realises'__step. }
+      apply WhileInduction. all:unfold R'__step,Rel';cbn.
       -intros t y tout. destruct Option.bind as [[] | ]eqn:Heq.
        3: intros (t1&b&Ht1&H);destruct b;[easy | ]; revert H.
        2:{ intros [Ht [= ->]]. all:hnf.
@@ -171,19 +172,19 @@ Module CheckEncodeList.
        split. easy. rewrite HcX. cbn. now autorewrite with list. *)
     Qed.
 
-    Lemma Terminates :
-      projT1 M ↓ (fun tin k => length (tape_local tin[@Fin0])*8 + 8 <= k).
+    Lemma Terminates' :
+      projT1 M' ↓ (fun tin k => length (tape_local tin[@Fin0])*8 + 8 <= k).
     Proof.
       cbn.
       eapply TerminatesIn_monotone.
-      { unfold M. TM_Correct_step.
-        2:eapply Terminates__step, RealiseIn_TerminatesIn.
-        1:eapply Realises__step. now apply @CheckEncodesBool.RealisesIn. }
+      { unfold M'. TM_Correct_step.
+        2:eapply Terminates'__step, RealiseIn_TerminatesIn.
+        1:eapply Realises'__step. now apply @CheckEncodesBool.RealisesIn. }
       eapply WhileCoInduction.
       intros tin k Hk. 
       infTer 4.
       intros [] tmid. now intros; nia.
-      cbn [R__step].  destruct Option.bind as [ [] | ] eqn:Hc. 1,2,4:intuition congruence.
+      cbn [R'__step].  destruct Option.bind as [ [] | ] eqn:Hc. 1,2,4:intuition congruence.
       intros (?&[]&Hbool&Ht'&H'&[=]). hnf in x. destruct_vector. cbn in Ht'. subst h. cbn - [plus] in *. 
       destruct (tin[@Fin0]) as [ | | | ? ? t__R]. 1-3:easy. cbn - [plus] in *. 
       destruct Hbool as [(x&Hx1&Hx2) _]. cbn in Hx1,Hx2.
@@ -193,51 +194,32 @@ Module CheckEncodeList.
       rewrite H'. rewrite tape_local_move_right'.
       eexists. split. reflexivity. nia.
     Qed.
+  End checkEncodesBoolList.
 
-    
-    (*
-    Context c__X (Terminates__X : projT1 M__X ↓ (ContainsEncoding.Ter cX Retr_f c__X)).
+  Section checkEncodesBoolList2.
+  Import Hoare.
 
-    
-    Variable c':nat.
-    (* This sems hard as the run-time depends on the precise values. *)
-    Lemma Terminates :
-      projT1 M ↓ ContainsEncoding.Ter (Encode_list cX) Retr_f c'.
-    Proof. (*
-      unfold M.
-      eapply TerminatesIn_monotone.
-      { TM_Correct_step. now apply Realises__step. apply Terminates__step. eassumption. }
-      apply WhileCoInduction.
-      intros tin k Ter__X.
-      assert (exists y, R__step tin y /\ forall y', R__step tin (None,y') -> y = (None,y')).
-      { destruct Ter__X as (k__X&?&?&?). edestruct Terminates__step. eassumption.  unfold ContainsEncoding.Ter. 
-        2:{eexists. split. eapply Realises__step. eassumption.
-           unfold R__step. intros ?. destruct Option.bind as [[] | ] eqn:eqc.  1,2,4:intuition congruence.
-           intros (?&[]&RX&?&?). 2:congruence. unfold Rel__X in RX.
-           eapply ContainsEncoding.functional_true in RX. 2-3:admit.
-        intros ? H'. eapply Realises__step in H. unfold R__step in *. }
-      (l&Htin&Hl&Hk).
-      -destruct (Encode_list _ x) eqn:eqxs. now destruct xs.
-       unfold ContainsEncoding.Ter. cbn - [R__step] in *. 
-       erewrite tape_local_move_right. 2:eassumption.  
-      do 2 eexists.
-      -eexists. split. 2:easy. applt cbn.
-      eexists. eapply Realises__step. eapply Switch_TerminatesIn. 1,2:now TM_Correct.
-        introsSwitch c. destructBoth c as [ [] | ]. all:TM_Correct. all:eassumption. }
-      intros ? ? HT. infTer 5.
-      2:{ intros t ? (?&->&->&<-).
-          destructBoth (Option.bind Retr_g (current t[@Fin0])) eqn. as [ | ].
-            infTer 5.  unfold CheckEncodesTape.Ter. intros ? _ Htout. rewrite !Htout. infTer 4.
-            intros ? ? ?. destruct b.
-            -infTer 5. intros ? ? ->.
-             rewrite !Ht. cbn in *. fold n0.  destruct H as [_ (k&H)].
-             rewrite H. rewrite iter_transitive with (g:=fun x => | right x |) (R:=le). 2:eauto. 2:apply Ht.
-             rewrite Htout,Ht. fold n0. reflexivity.
-            -nia.
-            -nia.
-             intros ? ? ?. nia. *)
-    Abort.
-*)
-  End checkEncodeList.
-End CheckEncodeList.
+    Context (Σ : finType) (retr__bools : Retract (sigList bool) Σ).
+    Definition M : pTM (Σ^+) bool 1 := CheckTapeContains.M (M' (I:=_)).
+
+    Lemma SpecT tape0:
+     TripleT (≃≃([ ],[|Custom (eq tape0)|]))
+        (12 * S(| right tape0 |) + 19) M 
+        (fun yout => ≃≃([inhabited (reflect (exists (bs:list bool), tape_contains _ tape0 bs) yout)]
+                        ,[|Custom (if yout then eq tape0 else fun _ => True)|])).
+    Proof.
+      unfold M. eapply Realise_TripleT.
+      - eapply CheckTapeContains.Realise. eapply Realise'. now intros []. now apply list_encode_prefixInjective,DecodeBool.bool_encode_prefixInjective.
+      - eapply CheckTapeContains.Terminates. { eapply Realise'. now intros []. }
+        eapply Terminates'.
+      - intros tin b tout H HEnc. cbn in *.
+        specialize (HEnc Fin0) as ->; simpl_vector in *; cbn in *.
+        destruct H,b;tspec_solve. all:firstorder subst;eauto.
+      - intros tin k HEnc Hk. cbn.
+        specialize (HEnc Fin0) as ->;simpl_vector in *;cbn - ["+" "*"] in *.
+        eexists;split. reflexivity.
+        rewrite <- Hk. destruct (tin[@Fin0]) as [| | | ? ? []];cbn - ["+" "*"];try nia.
+    Qed.
+  End checkEncodesBoolList2.
+End CheckEncodesBoolList.
 
