theories/L/Complexity/Reductions/Cook/tmp.v
@@ -1,8 +1,0 @@
-Require Import Lia.
-
-Goal forall n, n < 5 -> exists X, n + X = 5.
-  intros.
-  eexists; split.
-  - unfold "<". reflexivity.
-  - auto.
-Qed.
